Vernacular command for sigma unpacking

plugin/src/automation/unpack.ml
@@ -1,0 +1,49 @@
+open Util
+open Names
+open Libnames
+open Univ
+open Context
+(* open Pretyping *)
+open CErrors
+open Coqterms
+open Ltac_plugin
+
+let unpack_tactic =
+  Qualid (qualid_of_string "Ornamental.Unpack.unpack") |> CAst.make
+
+let unpack_term_tactic =
+  Qualid (qualid_of_string "Ornamental.Unpack.unpack_term") |> CAst.make
+
+let unpack_type_tactic =
+  Qualid (qualid_of_string "Ornamental.Unpack.unpack_type") |> CAst.make
+
+(* let tactify_expr e =
+ *   Tacexpr.ConstrMayEval (Genredexpr.ConstrTerm e) *)
+
+(* Evaluate a tactic on no goals and return any proofs constructed *)
+let eval_tactic env evm ?goal tac =
+  let typ, _ = Evarutil.e_new_type_evar env evm Evd.univ_flexible_alg in
+  let (ent, pv) = Proofview.init !evm [(env, typ)] in
+  let ((), pv, (unsafe, shelved, obliged), _) = Proofview.apply env tac pv in
+  evm := Proofview.proofview pv |> snd;
+  (* evm := TODO: solve_remaining_evars (default_inference_flags true) env evm evm0; *)
+  let proofs = Proofview.partial_proof ent pv |> List.map (EConstr.to_constr !evm) in
+  (* let shelved = List.filter (Evd.is_undefined !evm) shelved in
+   * let obliged = List.filter (Evd.is_undefined !evm) obliged in
+   * List.iter (Printer.pr_constr_env env !evm %> Feedback.msg_debug) proofs;
+   * List.map (Printer.pr_existential_key !evm) obliged |> Pp.seq |> Feedback.msg_debug;
+   * List.map (Printer.pr_existential_key !evm) shelved |> Pp.seq |> Feedback.msg_debug; *)
+  List.hd proofs
+
+let call_tactic env evm tac args =
+  let open Tacexpr in
+  let args = List.map (fun e -> ConstrMayEval (Genredexpr.ConstrTerm e)) args in
+  TacArg (Loc.tag (TacCall (Loc.tag (tac, args)))) |> Tacinterp.interp |>
+  eval_tactic env evm
+
+let unpack_constant env evm const =
+  let const_term = Evarutil.e_new_global evm (ConstRef const) in
+  let const_type = Typing.e_type_of env evm const_term in
+  call_tactic env evm unpack_term_tactic
+    [Constrextern.extern_constr false env !evm const_term;
+     Constrextern.extern_constr false env !evm const_type]
