plugin/src/automation/unpack.mli
@@ -1,0 +1,4 @@
+open Names
+open Constr
+
+val unpack_constant : Environ.env -> Evd.evar_map ref -> Constant.t -> constr
