plugin/theories/Ornaments.v
@@ -1,4 +1,4 @@
+Require Ornamental.Unpack.
 Require Ornamental.Lifted.
 
 Declare ML Module "ornaments".
-
