plugin/theories/Unpack.v
@@ -1,0 +1,234 @@
+Require Import Coq.Program.Tactics.
+Require Import Coq.Logic.EqdepFacts.
+
+Local Notation "( x ; y )" := (@existT _ _ x y).
+Local Notation "p '.1'" := (@projT1 _ _ p) (left associativity, at level 8).
+Local Notation "p '.2'" := (@projT2 _ _ p) (left associativity, at level 8).
+
+Lemma sigT_eta {A : Type} {B : A -> Type} (p : {x:A & B x}) : p = (p.1; p.2).
+Proof. destruct p. auto. Defined.
+
+Lemma eq_sigT_eta {A : Type} {B : A -> Type} {p q : {x:A & B x}} :
+  p = q -> (p.1; p.2) = (q.1; q.2).
+Proof. destruct p, q. auto. Defined.
+
+Ltac rewrap unwrapped :=
+  lazymatch goal with
+  | [ |- forall (x : ?A), @?C x ] =>
+    let x := fresh x in
+    refine (fun (x : ?A) => _);
+    lazymatch A with
+    | @sigT _ _ =>
+      rewrap (unwrapped x.1 x.2)
+    | _ =>
+      rewrap (unwrapped x)
+    end
+  | [ |- @eq_dep ?A ?B ?x_i ?x ?y_i ?y ] =>
+    exact (@eq_dep_eq_sigT A B x_i y_i x y unwrapped)
+  | [ |- _ ] =>
+    exact unwrapped
+  end.
+
+Ltac unwrap wrapped :=
+  lazymatch (eval hnf in wrapped) with
+  | forall (x : ?A), @?C x =>
+    let x := fresh x in
+    lazymatch A with
+    | @sigT ?A ?B =>
+      let x_i := fresh x "_i" in
+      refine (forall (x_i : A) (x : B x_i), _);
+      unwrap (C (x_i; x))
+    | _ =>
+      refine (forall (x : A), _);
+      unwrap (C x)
+    end
+  | @eq (@sigT ?A ?B) ?x ?y =>
+    exact (eq_dep A B x.1 x.2 y.1 y.2)
+  | _ =>
+    exact wrapped
+  end.
+
+Ltac repack index value :=
+  lazymatch goal with
+  | [ |- forall (x : ?A), _ ] =>
+    let x := fresh x in
+    refine (fun (x : ?A) => _);
+    lazymatch A with
+    | @sigT _ _ =>
+      repack (index x.1 x.2) (value x.1 x.2)
+    | _ =>
+      repack (index x) (value x)
+    end
+  | [ |- @sigT _ _ ] =>
+    exact (index; value)
+  end.
+
+Ltac unpack_index packed :=
+  lazymatch (eval hnf in packed) with
+  | forall (x : ?A), @?C x =>
+    let x := fresh x in
+    lazymatch A with
+    | @sigT ?A ?B =>
+      let x_i := fresh x "_i" in
+      refine (forall (x_i : A) (x : B x_i), _);
+      unpack_index (C (x_i; x))
+    | context K [(@sigT _ _)] =>
+      let A' := unwrap A in
+      refine (forall (x : A'), _);
+      assert A as x' by rewrap x;
+      unpack_index (C x')
+    | _ =>
+      refine (forall (x : A), _);
+      unpack_index (C x)
+    end
+  | @sigT ?A ?B =>
+    exact A
+  end.
+
+Ltac unpack_value packed index :=
+  lazymatch (eval hnf in packed) with
+  | forall (x : ?A), @?C x =>
+    let x := fresh x in
+    lazymatch A with
+    | @sigT ?A ?B =>
+      let x_i := fresh x "_i" in
+      refine (forall (x_i : A) (x : B x_i), _);
+      unpack_value (C (x_i; x) (index x_i x))
+    | context K [(@sigT _ _)] =>
+      let A' := unwrap A in
+      refine (forall (x : A'), _);
+      assert A as x' by rewrap x;
+      unpack_value (C x') (index x')
+    | _ =>
+      refine (forall (x : A), _);
+      unpack_value (C x) (index x)
+    end
+  | @sigT ?A ?B =>
+    exact (B index)
+  end.
+
+Ltac unpack_type t :=
+  lazymatch (eval hnf in t) with
+  | forall (x : @sigT ?A ?B), @?C x =>
+    let x := fresh x in
+    let x_i := fresh x "_i" in
+    refine (forall (x_i : A), _);
+    refine (forall (x : B x_i), _);
+    unpack_type (C (x_i; x))
+  | forall (x : ?A), @?C x =>
+    let x := fresh x in
+    lazymatch A with
+    | (@sigT ?A ?B) =>
+      let x_i := fresh x "_i" in
+      refine (forall (x_i : A), _);
+      refine (forall (x : B x_i), _);
+      unpack_type (C (x_i; x))
+    | context K [forall _, sigT _ _] =>
+      let x_i := fresh x "_i" in
+      let A' := unpack_index A in
+      refine (forall (x_i : A), _);
+      let B' := unpack_value A x_i in
+      refine (forall (x : B' x_i), _);
+      assert A as x' by repack x_i x;
+      unpack_type (C x')
+    | context K [forall (_ : sigT _ _), _] =>
+      let A' := unwrap A in
+      refine (forall (x : A'), _);
+      assert A as x' by rewrap x;
+      unpack_type (C x')
+    | _ =>
+      refine (forall (x : A), _);
+      unpack_type (C x)
+    end
+  | @eq (@sigT ?A ?B) ?x ?y =>
+    exact (eq_dep A B x.1 x.2 y.1 y.2)
+  | @sigT ?A ?B =>
+    refine (B ?[i]);
+    unshelve (instantiate (i := _))
+  | _ =>
+    exact t
+  end.
+
+(* NOTE: The current type doesn't really need to be another argument... *)
+Ltac unpack_term e t :=
+  lazymatch (eval hnf in t) with
+  | forall (x : @sigT ?A ?B), @?C x =>
+    let x := fresh x in
+    let x_i := fresh x "_i" in
+    refine (fun (x_i : A) (x : B x_i) => _);
+    unpack_term (e (x_i; x)) (C (x_i; x))
+  | forall (x : ?A), @?C x =>
+    let x := fresh x in
+    lazymatch A with
+    | (@sigT ?A ?B) =>
+      let x_i := fresh x "_i" in
+      refine (fun (x_i : A) => _);
+      refine (fun (x : B x_i) => _);
+      unpack_term (e (x_i; x)) (C (x_i; x))
+    | context K [forall _, sigT _ _] =>
+      let x_i := fresh x "_i" in
+      let A' := unpack_index A in
+      refine (fun (x_i : A) => _);
+      let B' := unpack_value A x_i in
+      refine (fun (x : B' x_i) => _);
+      assert A as x' by repack x_i x;
+      unpack_term (e x') (C x')
+    | context K [forall (_ : sigT _ _), _] =>
+      let A' := unwrap A in
+      refine (fun (x : A') => _);
+      assert A as x' by rewrap x;
+      unpack_term (e x') (C x')
+    | _ =>
+      refine (fun (x : A) => _);
+      unpack_term (e x) (C x)
+    end
+  | @eq (@sigT ?A ?B) ?x ?y =>
+    refine (eq_sigT_eq_dep A B x.1 y.1 x.2 y.2 (eq_sigT_eta e))
+  | @sigT ?A ?B =>
+    exact (e.2)
+  | _ =>
+    exact e
+  end.
+
+(* NOTE: The current type doesn't really need to be another argument... *)
+Ltac unpack e :=
+  lazymatch (eval hnf in ltac:(type of e)) with
+  | forall (x : @sigT ?A ?B), @?C x =>
+    let x := fresh x in
+    let x_i := fresh x "_i" in
+    refine (fun (x_i : A) (x : B x_i) => _);
+    unpack (e (x_i; x))
+  | forall (x : ?A), @?C x =>
+    let x := fresh x in
+    lazymatch A with
+    | (@sigT ?A ?B) =>
+      let x_i := fresh x "_i" in
+      refine (fun (x_i : A) => _);
+      refine (fun (x : B x_i) => _);
+      unpack (e (x_i; x))
+    | context K [forall _, sigT _ _] =>
+      let x_i := fresh x "_i" in
+      let A' := unpack_index A in
+      refine (fun (x_i : A) => _);
+      let B' := unpack_value A x_i in
+      refine (fun (x : B' x_i) => _);
+      assert A as x' by repack x_i x;
+      unpack (e x')
+    | context K [forall (_ : sigT _ _), _] =>
+      let A' := unwrap A in
+      refine (fun (x : A') => _);
+      assert A as x' by rewrap x;
+      unpack (e x')
+    | _ =>
+      refine (fun (x : A) => _);
+      unpack (e x)
+    end
+  | @eq (@sigT ?A ?B) ?x ?y =>
+    refine (eq_sigT_eq_dep A B x.1 y.1 x.2 y.2 (eq_sigT_eta e))
+  | @sigT ?A ?B =>
+    exact (e.2)
+  | _ =>
+    exact e
+  end.
+
+(* Ltac unpack e := unpack_term e ltac:(type of e). *)
